Invariant/ValidAttacker/ValidAttackerII/OneStepPreservesValidAttackerII.v
@@ -17,6 +17,7 @@ Require Import Invariant.ValidAttacker.ValidAttackerII.ExploitationRemoteService
 Require Import Invariant.ValidAttacker.ValidAttackerII.RemoteSystemDiscovery.
 Require Import Invariant.ValidAttacker.ValidAttackerII.SystemServiceDiscovery.
 Require Import Invariant.ValidAttacker.ValidAttackerII.FileDirectoryDiscoveryLocal.
+Require Import Invariant.ValidAttacker.ValidAttackerII.UnsecuredCredentials.
 
 Theorem one_step_preserves_valid_attacker_ii : forall (a a' : Attacker) (t : Technique) (n: network_map),
       one_step a t n a' -> valid_attacker_ii a'.
@@ -27,7 +28,7 @@ Theorem one_step_preserves_valid_attacker_ii : forall (a a' : Attacker) (t : Tec
     unfold Pre in H1; unfold Post in H2; unfold valid_attacker_ii.
     - apply (one_step_remote_services_preserves_valid_attacker_ii a a' network H0 i i1 i0 i2 k i3); auto.
     - apply (one_step_exploitation_remote_services_preserves_valid_attacker_ii a a' network H0 i i1 i0 i2 i3); auto.
-    - admit. (* Unsecured_Credentials *)
+    - apply (one_step_unsecured_credentials_preserves_valid_attacker_ii a a' network H0 i i0 i1); auto. (* Unsecured_Credentials *)
     - admit. (* Brute_Force *)
     - admit. (* Abuse_Elevation_Control_Mechanism *)
     - apply (one_step_file_directory_discovery_local_preserves_valid_attacker_ii a a' network H0 i i0 p); auto.
