Invariant/ValidAttacker/ValidAttackerII/UnsecuredCredentials.v
@@ -1,0 +1,78 @@
+Require Import Coq.Lists.List.
+
+Require Import Machine.Machine.
+Require Import Machine.MachineValid.
+Require Import Machine.MachineAuxFunctions.
+Require Import Attacker.Attacker.
+Require Import Technique.Technique.
+Require Import Technique.TechniquePreCondition.
+Require Import Technique.TechniquePostCondition.
+
+Require Import Invariant.AuxLemmas.AuxLemmas.
+Require Import Invariant.AuxTactics.
+
+Lemma one_step_unsecured_credentials_preserves_valid_attacker_ii : forall (a a' : Attacker) (n: network_map) (aValid: valid_attacker a n) (m : idMachine) (u : idUser) (s: idService),
+      valid_concrete_network n -> Pre a (Unsecured_Credentials m u s) -> Post a (Unsecured_Credentials m u s) n a' -> valid_attacker_ii a'.
+  Proof.
+    intros a a' network validAttacker m u s validNetwork pre post.
+    unfold valid_attacker_ii.
+    intros m0 p0 H_secrets_a'.
+    unfold valid_attacker in validAttacker.
+    elim validAttacker.
+    elim_intro_clear validAttacker validAttackerI validAttacker'.
+    elim_intro_clear validAttacker' validAttackerII validAttacker''.
+    unfold Pre in pre; destruct post.
+
+    elim_intro_clear H0 Hsecrets H0'.
+    elim_intro_clear H0' mac H0.
+    elim_intro_clear H0 macView H0'.
+    elim_intro_clear H0' newMacView H0.
+    elim_intro_clear H0 accs H0'.
+    elim_intro_clear H0' accsView H0.
+    elim_intro_clear H0 accsLinkedToUser H0'.
+    elim_intro_clear H0' accsNewView H0.
+    elim_intro_clear H0 accView H1.
+
+    elim_intro_clear H1 env_m H1'.
+    elim_intro_clear H1' network_m H1.
+    elim_intro_clear H1 accsView_eq H1'.
+    elim_intro_clear H1' accView_in H1.
+    elim_intro_clear H1 accView_user H1'.
+    elim_intro_clear H1' accView_service H1.
+    elim_intro_clear H1 accs_mac H1'.
+    elim_intro_clear H1' accsLinked_eq H1.
+    elim_intro_clear H1 accsNewView_eq H1'.
+    elim_intro_clear H1' newMacView_eq env_a'.
+
+    unfold valid_attacker_ii in validAttackerII.
+    elim (validAttackerII m0 p0).
+    intros MAC IH.
+    elim_intro_clear IH env_MAC path_MAC.
+    - case (idMachine_eq m0 m); intro eq_m0.
+      -- exists newMacView.
+         split.
+         --- rewrite env_a'.
+             unfold modify_machine.
+             case (idMachine_eq m0 m); intros.
+             ---- reflexivity.
+             ---- contradiction.
+         --- unfold registered_paths.
+             rewrite newMacView_eq.
+             simpl.
+             assert (macView = MAC).
+             ---- apply (enviroment_map_image (enviroment a) m macView MAC).
+                  ----- exact env_m.
+                  ----- rewrite <- eq_m0. exact env_MAC.
+             ---- unfold registered_paths in path_MAC.
+                  rewrite <- H2 in path_MAC.
+                  exact path_MAC.
+      -- exists MAC.
+         rewrite (enviroment_eq (enviroment a) (enviroment a') m0 m newMacView).
+         --- split.
+             ---- exact env_MAC.
+             ---- exact path_MAC.
+         --- exact eq_m0.
+         --- exact env_a'.
+    - rewrite Hsecrets in H_secrets_a'.
+      exact H_secrets_a'.
+  Qed.
