Invariant/ValidAttacker/ValidAttackerIII/UnsecuredCredentials.v
@@ -1,0 +1,155 @@
+Require Import Coq.Lists.List.
+
+Require Import Machine.Machine.
+Require Import Machine.MachineValid.
+Require Import Machine.MachineAuxFunctions.
+Require Import Attacker.Attacker.
+Require Import Technique.Technique.
+Require Import Technique.TechniquePreCondition.
+Require Import Technique.TechniquePostCondition.
+
+Require Import Invariant.AuxLemmas.AuxLemmas.
+Require Import Invariant.AuxTactics.
+
+Lemma one_step_unsecured_credentials_preserves_valid_attacker_iii : forall (a a' : Attacker) (n: network_map) (aValid: valid_attacker a n) (m : idMachine) (u : idUser) (s: idService),
+      valid_concrete_network n -> Pre a (Unsecured_Credentials m u s) -> Post a (Unsecured_Credentials m u s) n a' -> valid_attacker_iii a'.
+  Proof.
+    intros a a' network validAttacker m u s validNetwork pre post.
+    unfold valid_attacker_iii.
+    unfold valid_network.
+    elim_intro_clear validAttacker validAttackerI validAttacker'.
+    elim_intro_clear validAttacker' validAttackerII validAttacker''.
+    elim_intro_clear validAttacker'' validAttackerIII validAttackerIV.
+    unfold Pre in pre; destruct post.
+    clear validNetwork validAttackerI validAttackerII validAttackerIV.
+
+    elim_intro_clear H0 Hsecrets H0'.
+    elim_intro_clear H0' mac H0.
+    elim_intro_clear H0 macView H0'.
+    elim_intro_clear H0' newMacView H0.
+    elim_intro_clear H0 accs H0'.
+    elim_intro_clear H0' accsView H0.
+    elim_intro_clear H0 accsLinkedToUser H0'.
+    elim_intro_clear H0' accsNewView H0.
+    elim_intro_clear H0 accView H1.
+
+    elim_intro_clear H1 env_m H1'.
+    elim_intro_clear H1' network_m H1.
+    elim_intro_clear H1 accsView_eq H1'.
+    elim_intro_clear H1' accView_in H1.
+    elim_intro_clear H1 accView_user H1'.
+    elim_intro_clear H1' accView_service H1.
+    elim_intro_clear H1 accs_mac H1'.
+    elim_intro_clear H1' accsLinked_eq H1.
+    elim_intro_clear H1 accsNewView_eq H1'.
+    elim_intro_clear H1' newMacView_eq env_a'.
+
+    unfold valid_attacker_iii in validAttackerIII.
+    unfold valid_network in validAttackerIII.
+    elim_intro_clear validAttackerIII network_top_enva valid_machine_enva.
+    unfold network_topology in *.
+    split.
+    - intros.
+      rewrite env_a'.
+      unfold modify_machine.
+      case (idMachine_eq neighbour m); case (idMachine_eq mid m); intros eq_mid eq_neigh.
+      -- exists newMacView; auto.
+      -- exists newMacView; auto.
+      -- apply (network_top_enva m neighbour macView).
+         --- intro contra. symmetry in contra. exact (eq_neigh contra).
+         --- exact env_m.
+         --- assert (Heq_m0: m0 = newMacView).
+             ---- apply (enviroment_simpl (enviroment a) (enviroment a') mid m).
+                  ----- exact eq_mid.
+                  ----- exact env_a'.
+                  ----- exact H1.
+             ---- rewrite Heq_m0 in H2.
+                  rewrite newMacView_eq in H2.
+                  unfold is_neighbour in *.
+                  simpl in H2.
+                  exact H2.
+      -- apply (network_top_enva mid neighbour m0).
+         --- exact H0.
+         --- rewrite <- (enviroment_eq (enviroment a) (enviroment a') mid m newMacView).
+             ---- exact H1.
+             ---- exact eq_mid.
+             ---- exact env_a'.
+         --- exact H2.
+    - intros.
+      case (idMachine_eq mid m); intros eq_m.
+      -- assert (m0 = newMacView).
+         apply (enviroment_simpl (enviroment a) (enviroment a') mid m).
+         --- exact eq_m.
+         --- exact env_a'.
+         --- exact H0.
+         --- rewrite H1.
+             elim (valid_machine_enva m macView).
+             intros.
+             elim_intro_clear H3 H6 H5.
+             elim_intro_clear H5 H7 H8.
+             unfold valid_machine.
+             rewrite newMacView_eq.
+             split.
+             ---- unfold users_access_to_files in *.
+                  unfold registered_users in *.
+                  simpl.
+                  rewrite accsNewView_eq.
+                  rewrite <- accsView_eq.
+                  intros f Hinf.
+                  destruct (H2 f Hinf) as [Hacc_user H5].
+                  destruct H5 as [ Hacc Hin_f].
+                  destruct Hacc as [acc Hacc'].
+                  destruct Hacc' as [ Heq_acc Hin_acc ].
+                  ----- exists Hacc_user.
+                        split.
+                        ------ apply oplusAccounts_preserves_registered_user.
+                               exists acc.
+                               split.
+                               ------- exact Heq_acc.
+                               ------- exact Hin_acc.
+                        ------ exact Hin_f.
+             ---- split.
+                  ----- unfold users_access_to_services in *.
+                        unfold registered_service in *.
+                        simpl.
+                        intros acc0 HIP.
+                        rewrite accsNewView_eq in HIP.
+                        apply member_oplusAccounts_simpl in HIP.
+                        destruct HIP as [HIP | HIP].
+                        ------ (* acc0 proviene de accsLinkedToUser *)
+                               right.
+                               assert (Hservice: account_service acc0 = Some s).
+                               { rewrite accsLinked_eq in HIP.
+                                 apply (get_accounts_linked_service_with_key_service u s accs).
+                                 exact HIP. }
+                               exists s.
+                               split.
+                               ------- exact Hservice.
+                               ------- assert (Hin_accView: In accView (machine_accounts macView)).
+                                       { rewrite accsView_eq. exact accView_in. }
+                                       destruct (H6 accView Hin_accView) as [Habs | [s0 [Hs0 Hserv]]].
+                                       -------- rewrite accView_service in Habs. discriminate.
+                                       -------- rewrite accView_service in Hs0.
+                                                injection Hs0 as Hs0.
+                                                rewrite <- Hs0 in Hserv.
+                                                exact Hserv.
+                        ------ (* acc0 proviene de accsView *)
+                               rewrite <- accsView_eq in HIP.
+                               apply H6. exact HIP.
+                  ----- unfold valid_fileSystem.
+                        simpl.
+                        split.
+                        ------ unfold subfiles_in_machine in *. 
+                               unfold registered_paths in *.
+                               simpl in *.
+                               exact H7.
+                        ------ exact H8.
+             ---- exact env_m.
+      -- assert (enviroment a' mid = enviroment a mid).
+         apply (enviroment_eq (enviroment a) (enviroment a') mid m newMacView).
+         --- exact eq_m.
+         --- exact env_a'.
+         --- rewrite H1 in H0.
+             apply (valid_machine_enva mid m0).
+             exact H0.
+  Qed.
