Invariant/ValidAttacker/ValidAttackerIV/UnsecuredCredentials.v
@@ -1,0 +1,119 @@
+Require Import Coq.Lists.List.
+
+Require Import Machine.Machine.
+Require Import Machine.MachineValid.
+Require Import Machine.MachineAuxFunctions.
+Require Import Machine.MachineView.
+
+Require Import Attacker.Attacker.
+
+Require Import Technique.Technique.
+Require Import Technique.TechniquePreCondition.
+Require Import Technique.TechniquePostCondition.
+
+Require Import Invariant.AuxLemmas.AuxLemmas.
+Require Import Invariant.AuxTactics.
+
+Lemma one_step_unsecured_credentials_preserves_valid_attacker_iv : forall (a a' : Attacker) (n: network_map) (aValid: valid_attacker a n) (m : idMachine) (u : idUser) (s: idService),
+      valid_concrete_network n -> Pre a (Unsecured_Credentials m u s) -> Post a (Unsecured_Credentials m u s) n a' -> valid_attacker_iv a' n.
+  Proof.
+    intros a a' network validAttacker m u s validNetwork pre post.
+    unfold valid_attacker_iv.
+    unfold is_networkView.
+    elim_intro_clear validAttacker validAttackerI validAttacker'.
+    elim_intro_clear validAttacker' validAttackerII validAttacker''.
+    elim_intro_clear validAttacker'' validAttackerIII validAttackerIV.
+    unfold Pre in pre; destruct post.
+    clear validAttackerI validAttackerII validAttackerIII.
+
+    elim_intro_clear H0 Hsecrets H0'.
+    elim_intro_clear H0' mac H0.
+    elim_intro_clear H0 macView H0'.
+    elim_intro_clear H0' newMacView H0.
+    elim_intro_clear H0 accs H0'.
+    elim_intro_clear H0' accsView H0.
+    elim_intro_clear H0 accsLinkedToUser H0'.
+    elim_intro_clear H0' accsNewView H0.
+    elim_intro_clear H0 accView H1.
+
+    elim_intro_clear H1 env_m H1'.
+    elim_intro_clear H1' network_m H1.
+    elim_intro_clear H1 accsView_eq H1'.
+    elim_intro_clear H1' accView_in H1.
+    elim_intro_clear H1 accView_user H1'.
+    elim_intro_clear H1' accView_service H1.
+    elim_intro_clear H1 accs_mac H1'.
+    elim_intro_clear H1' accsLinked_eq H1.
+    elim_intro_clear H1 accsNewView_eq H1'.
+    elim_intro_clear H1' newMacView_eq env_a'.
+
+    unfold valid_attacker_iv in validAttackerIV.
+    unfold is_networkView in validAttackerIV.
+    intros m0 mac1 mac2 env_a'_m0 network_m0.
+    unfold is_machineView.
+    case (idMachine_eq m0 m); intros eq_m0.
+    elim (validAttackerIV m0 macView mac).
+    intros Hserv. intro Hserv'.
+    destruct Hserv' as [Haccs Hserv'']. 
+    destruct Hserv'' as [Hfiles Hneighs].
+    assert (Heq_mac1: mac1 = newMacView).
+    {
+      apply (enviroment_simpl (enviroment a) (enviroment a') m0 m mac1 newMacView).
+      - exact eq_m0.
+      - exact env_a'.
+      - exact env_a'_m0.
+    }
+    assert (Heq_mac2: mac2 = mac).
+    {
+      apply (enviroment_map_image network m mac2 mac).
+      - rewrite eq_m0 in network_m0. exact network_m0.
+      - exact network_m.
+    }
+    rewrite Heq_mac1.
+    rewrite Heq_mac2.   
+    split; [|split]; try split.
+    - unfold subset_services in *.
+      rewrite newMacView_eq.
+      simpl.
+      exact Hserv.
+    - unfold subset_accounts in *.
+      rewrite newMacView_eq.
+      simpl.
+      rewrite accsNewView_eq.
+      intros Hacc Hin_oplus.
+      apply member_oplusAccounts_simpl in Hin_oplus.
+      destruct Hin_oplus as [Hin_linked | Hin_accsView].
+      -- (* Hacc proviene de accsLinkedToUser: esta en machine_accounts mac *)
+         left.
+         rewrite accsLinked_eq in Hin_linked.
+         rewrite accs_mac.
+         apply (get_accounts_linked_service_with_key_in u s accs).
+         exact Hin_linked.
+      -- (* Hacc proviene de accsView: usar hipotesis Haccs *)
+         rewrite <- accsView_eq in Hin_accsView.
+         apply Haccs. exact Hin_accsView.
+    - unfold subset_files in *.
+      rewrite newMacView_eq.
+      simpl.
+      exact Hfiles.
+    - unfold subset_neighbours in *.
+      rewrite newMacView_eq.
+      simpl.
+      exact Hneighs.
+    - rewrite <- eq_m0 in env_m. exact env_m.
+    - rewrite <- eq_m0 in network_m. exact network_m.
+    - elim (validAttackerIV m0 mac1 mac2).
+      intros Hserv. intro Hserv'.
+      destruct Hserv' as [Haccs Hserv''].
+      destruct Hserv'' as [Hfiles Hneighs].
+      split; [|split]; try split.
+      -- exact Hserv.
+      -- exact Haccs.
+      -- exact Hfiles.
+      -- exact Hneighs.
+      -- rewrite <- (enviroment_eq (enviroment a) (enviroment a') m0 m newMacView).
+         --- exact env_a'_m0.
+         --- exact eq_m0.
+         --- exact env_a'.
+      -- exact network_m0.
+  Qed.
